Add function to run a trace entry

vyperTestRunnerScript.sml
@@ -52,8 +52,9 @@ Definition compute_selector_names_def:
   compute_selector_names (Function x::ls) =
   let name = x.name in
   let argTypes = MAP SND x.inputs in
+  let retTypes = MAP SND x.outputs in
   let sel = function_selector name argTypes in
-    (sel, name, argTypes)::compute_selector_names ls
+    (sel, name, argTypes, retTypes)::compute_selector_names ls
 End
 
 val () = cv_auto_trans compute_selector_names_def;
@@ -76,9 +77,9 @@ Datatype:
 End
 
 Definition find_function_args_by_name_def:
-  find_function_args_by_name n [] = [] ∧
-  find_function_args_by_name n (FunctionDecl _ _ id args _ _ :: ts) =
-  (if n = id then args else find_function_args_by_name n ts) ∧
+  find_function_args_by_name n [] = ([], NoneT) ∧
+  find_function_args_by_name n (FunctionDecl _ _ id args ret _ :: ts) =
+  (if n = id then (args, ret) else find_function_args_by_name n ts) ∧
   find_function_args_by_name n (_ :: ts) =
   find_function_args_by_name n ts
 End
@@ -86,27 +87,30 @@ End
 Definition compute_vyper_args_def:
   compute_vyper_args ts name argTys cd = let
     abiArgsTup = dec (Tuple argTys) cd;
-    vyTys = MAP SND $ find_function_args_by_name name ts;
+    argsret = find_function_args_by_name name ts;
+    args = FST argsret;
+    vyTys = MAP SND $ args;
     vyArgsTup = abi_to_vyper (TupleT vyTys) abiArgsTup;
+    vyArgs = (case OPTION_BIND vyArgsTup extract_elements
+                of NONE => [] | SOME ls => ls)
   in
-    case OPTION_BIND vyArgsTup extract_elements
-      of NONE => [] | SOME ls => ls
+    (vyArgs, SND argsret)
 End
 
 Definition run_deployment_def:
   run_deployment am dt = let
     sns = compute_selector_names dt.contractAbi;
     sel = TAKE 4 dt.callData;
-    fna = case ALOOKUP sns sel of SOME fna => fna | NONE => ("__init__", []);
-    name = FST fna; argTys = SND fna;
+    fna = case ALOOKUP sns sel of SOME fna => fna
+             | NONE => ("__init__", [], []);
+    name = FST fna; argTys = FST (SND fna);
     tx = <| sender := dt.deployer
           ; target := dt.deployedAddress
           ; function_name := name
-          ; args := compute_vyper_args dt.sourceAst name
-                      argTys (DROP 4 dt.callData)
+          ; args := FST $ compute_vyper_args dt.sourceAst
+                          name argTys (DROP 4 dt.callData)
           ; value := dt.value |>;
   in (sns, load_contract am tx dt.sourceAst)
-  (* TODO: check dt.deploymentSuccess *)
 End
 
 val () = cv_auto_trans run_deployment_def;
@@ -114,17 +118,69 @@ val () = cv_auto_trans run_deployment_def;
 Definition run_call_def:
   run_call sns am ct = let
     sel = TAKE 4 ct.callData;
-    fna = case ALOOKUP sns sel of SOME fna => fna | NONE => ("__default__", []);
-    name = FST fna; argTys = SND fna;
+    fna = case ALOOKUP sns sel of SOME fna => fna
+             | NONE => ("__default__", [], []);
+    name = FST fna; argTys = FST (SND fna);
     ts = case ALOOKUP am.sources ct.target of SOME ts => ts | _ => [];
+    ar = compute_vyper_args ts name argTys (DROP 4 ct.callData);
     tx = <| sender := ct.sender
           ; target := ct.target
           ; function_name := name
-          ; args := compute_vyper_args ts name argTys (DROP 4 ct.callData)
+          ; args := FST ar
           ; value := ct.value |>;
-  in call_external am tx
+  (* TODO: set static based on ct.static *)
+  (* TODO: set env data somewhere? *)
+  in (call_external am tx, (SND (SND fna), SND ar))
 End
 
 val () = cv_auto_trans run_call_def;
+
+Definition run_trace_def:
+  run_trace snss am tr =
+  case tr
+  of Deployment dt => let
+      result = run_deployment am dt;
+      sns = FST result;
+      snss = (dt.deployedAddress,sns)::snss;
+    in
+      (snss, SND result)
+   | Call ct => (snss,
+     case ALOOKUP snss ct.target
+     of NONE => if IS_NONE ct.expectedOutput then INL am
+                else INR (Error "sns not found")
+      | SOME sns => let
+        cr = run_call sns am ct;
+        call_res = FST cr;
+        am = SND call_res in
+       case FST call_res
+       of (* TODO: maybe AssertException is ok though? *)
+       | INR ex => if IS_NONE ct.expectedOutput then INL am
+                   else INR ex
+       | INL v =>
+       case ct.expectedOutput
+         of NONE => INR (Error "error expected")
+          | SOME out => let
+              rets = SND cr;
+              abiRetTys = FST rets;
+              abiRetTy = if NULL abiRetTys
+                         then Tuple []
+                         else HD abiRetTys; (* TODO: could there be multiple? *)
+              vyRetTy = SND rets;
+              abiret = dec abiRetTy out;
+              vyret = abi_to_vyper vyRetTy abiret;
+            in
+              if vyret = SOME v
+              then INL am
+              else INR (Error "output mismatch"))
+End
+
+val run_trace_pre_def = cv_auto_trans_pre run_trace_def;
+
+Theorem run_trace_pre[cv_pre]:
+  run_trace_pre x y z
+Proof
+  rw[run_trace_pre_def]
+  \\ strip_tac \\ gvs[]
+QED
 
 val () = export_theory();
